plugins/zify/zify.mli
@@ -1,0 +1,29 @@
+(************************************************************************)
+(*         *   The Coq Proof Assistant / The Coq Development Team       *)
+(*  v      *   INRIA, CNRS and contributors - Copyright 1999-2019       *)
+(* <O___,, *       (see CREDITS file for the list of authors)           *)
+(*   \VV/  **************************************************************)
+(*    //   *    This file is distributed under the terms of the         *)
+(*         *     GNU Lesser General Public License Version 2.1          *)
+(*         *     (see LICENSE file for the text of the license)         *)
+(************************************************************************)
+open Constrexpr
+module InjTable : sig val register : constr_expr -> unit end
+module UnOp     : sig val register : constr_expr -> unit end
+module BinOp    : sig val register : constr_expr -> unit end
+module CstOp    : sig val register : constr_expr -> unit end
+module BinRel   : sig val register : constr_expr -> unit end
+module PropOp   : sig val register : constr_expr -> unit end
+module Spec     : sig val register : constr_expr -> unit end
+module Saturate : sig val register : constr_expr -> unit end
+
+val zify_tac : unit Proofview.tactic
+val saturate : unit Proofview.tactic
+val iter_specs : (EConstr.t -> unit Proofview.tactic) -> unit Proofview.tactic
+
+val print_zify_types : unit -> unit
+val print_zify_binop : unit -> unit
+val print_zify_unop  : unit -> unit
+val print_zify_cst   : unit -> unit
+val print_zify_binrel: unit -> unit
+val print_zify_spec  : unit -> unit
