plugins/micromega/Tauto.v
@@ -253,6 +253,29 @@ Section S.
      *)
     Definition TFormula (TX: Type) (AF: Type) := @GFormula Term TX Annot AF.
 
+
+    Definition is_cnf_tt (c : cnf) : bool :=
+      match c with
+      | nil => true
+      | _  => false
+      end.
+
+    Definition is_cnf_ff (c : cnf) : bool :=
+      match c with
+      | nil::nil => true
+      | _        => false
+      end.
+
+    Definition and_cnf_opt (f1 : cnf) (f2 : cnf) : cnf :=
+      if is_cnf_ff f1 || is_cnf_ff f2
+      then cnf_ff
+      else and_cnf f1 f2.
+
+    Definition or_cnf_opt (f1 : cnf) (f2 : cnf) : cnf :=
+      if is_cnf_tt f1 || is_cnf_tt f2
+      then cnf_tt
+      else or_cnf f1 f2.
+
     Fixpoint xcnf {TX AF: Type} (pol : bool) (f : TFormula TX AF)  {struct f}: cnf :=
       match f with
       | TT  => if pol then cnf_tt else cnf_ff
@@ -261,10 +284,10 @@ Section S.
       | A x t => if pol then normalise x  t else negate x  t
       | N e  => xcnf (negb pol) e
       | Cj e1 e2 =>
-        (if pol then and_cnf else or_cnf) (xcnf pol e1) (xcnf pol e2)
-      | D e1 e2  => (if pol then or_cnf else and_cnf) (xcnf pol e1) (xcnf pol e2)
+        (if pol then and_cnf_opt else or_cnf_opt) (xcnf pol e1) (xcnf pol e2)
+      | D e1 e2  => (if pol then or_cnf_opt else and_cnf_opt) (xcnf pol e1) (xcnf pol e2)
       | I e1 _ e2
-        => (if pol then or_cnf else and_cnf) (xcnf (negb pol) e1) (xcnf pol e2)
+        =>  (if pol then or_cnf_opt else and_cnf_opt) (xcnf (negb pol) e1) (xcnf pol e2)
       end.
 
     Section CNFAnnot.
@@ -318,7 +341,7 @@ Section S.
         end.
 
 
-      Fixpoint ror_cnf f f' :=
+      Fixpoint ror_cnf (f f':list clause) :=
         match f with
         | nil => (cnf_tt,nil)
         | e :: rst =>
@@ -327,17 +350,23 @@ Section S.
           (rst_f' +++ e_f', t +++ t')
         end.
 
-      Definition is_cnf_tt (c : cnf) : bool :=
-        match c with
-        | nil => true
-        | _  => false
-        end.
+      Definition annot_of_clause (l : clause) : list Annot :=
+        List.map snd l.
 
-      Definition is_cnf_ff (c : cnf) : bool :=
-        match c with
-        | nil::nil => true
-        | _        => false
-        end.
+      Definition annot_of_cnf (f : cnf) : list Annot :=
+        List.fold_left (fun acc e => annot_of_clause e +++ acc ) f nil.
+
+
+      Definition ror_cnf_opt f1 f2 :=
+        if is_cnf_tt f1
+        then (cnf_tt ,  annot_of_cnf f1)
+        else if is_cnf_tt f2
+             then (cnf_tt, annot_of_cnf f2)
+             else ror_cnf f1 f2.
+
+
+
+
 
       Definition is_ff_no_deps_id {AF : Type} (e : cnf) (l : list Annot) (h : list AF) :=
         if is_cnf_ff e
@@ -354,27 +383,32 @@ Section S.
         | Some e => e ::l
         end.
 
+      Definition ratom {AF : Type}  (c : cnf) (a : Annot) : cnf * list Annot * list AF :=
+        if is_cnf_ff c || is_cnf_tt c
+        then (c,a::nil,nil)
+        else (c,nil,nil). (* t is embedded in c *)
+
       Fixpoint rxcnf {TX AF: Type}(polarity : bool) (f : TFormula TX AF) : cnf * list Annot * list AF:=
         match f with
         | TT => if polarity then (cnf_tt,nil,nil) else (cnf_ff,nil,nil)
         | FF  => if polarity then (cnf_ff,nil,nil) else (cnf_tt,nil,nil)
         | X p => if polarity then (cnf_ff,nil,nil) else (cnf_ff,nil,nil)
-        | A x t  => ((if polarity then normalise x t else negate x t),nil,nil)
+        | A x t  => ratom (if polarity then normalise x t else negate x t) t
         | N e  => rxcnf (negb polarity) e
         | Cj e1 e2 =>
           let '(e1,t1,h1) := rxcnf polarity e1 in
           let '(e2,t2,h2) := rxcnf polarity e2 in
           if polarity
-          then  (e1 +++ e2, t1 +++ t2,h1+++h2)
-          else let (f',t') := ror_cnf e1 e2 in
+          then  (and_cnf_opt e1  e2, t1 +++ t2,h1+++h2)
+          else let (f',t') := ror_cnf_opt e1 e2 in
             (f', t1 +++ t2 +++ t',h1+++h2)
         | D e1 e2  =>
           let '(e1,t1,h1) := rxcnf polarity e1 in
           let '(e2,t2,h2) := rxcnf polarity e2 in
           if polarity
-       then let (f',t') := ror_cnf e1 e2 in
+       then let (f',t') := ror_cnf_opt e1 e2 in
             (f', t1 +++ t2 +++ t',h1+++h2)
-          else (e1 +++ e2, t1 +++ t2,h1+++h2)
+          else (and_cnf_opt e1 e2, t1 +++ t2,h1+++h2)
         | I e1 a e2 =>
           let '(e1 , t1, h1) := (rxcnf (negb polarity) e1) in
           if polarity
@@ -384,12 +418,53 @@ Section S.
               rxcnf polarity e2
             else (* compute disjunction *)
               let '(e2 , t2, h2) := (rxcnf polarity e2) in
-              let (f',t') := ror_cnf e1 e2 in
+              let (f',t') := ror_cnf_opt e1 e2 in
               (f', t1 +++ t2 +++ t',ocons a (h1+++h2)) (* record the hypothesis *)
           else
             let '(e2 , t2, h2) := (rxcnf polarity e2) in
-            (and_cnf e1 e2, t1 +++ t2,h1+++h2)
+            (and_cnf_opt e1 e2, t1 +++ t2,h1+++h2)
         end.
+
+      Lemma rxcnf_rew {TX AF: Type}(polarity : bool) (f : TFormula TX AF) :
+        rxcnf  polarity f =
+        match f with
+        | TT => if polarity then (cnf_tt,nil,nil) else (cnf_ff,nil,nil)
+        | FF  => if polarity then (cnf_ff,nil,nil) else (cnf_tt,nil,nil)
+        | X p => if polarity then (cnf_ff,nil,nil) else (cnf_ff,nil,nil)
+        | A x t  => ratom (if polarity then normalise x t else negate x t) t
+        | N e  => rxcnf (negb polarity) e
+        | Cj e1 e2 =>
+          let '(e1,t1,h1) := rxcnf polarity e1 in
+          let '(e2,t2,h2) := rxcnf polarity e2 in
+          if polarity
+          then  (and_cnf_opt e1  e2, t1 +++ t2,h1+++h2)
+          else let (f',t') := ror_cnf_opt e1 e2 in
+            (f', t1 +++ t2 +++ t',h1+++h2)
+        | D e1 e2  =>
+          let '(e1,t1,h1) := rxcnf polarity e1 in
+          let '(e2,t2,h2) := rxcnf polarity e2 in
+          if polarity
+       then let (f',t') := ror_cnf_opt e1 e2 in
+            (f', t1 +++ t2 +++ t',h1+++h2)
+          else (and_cnf_opt e1 e2, t1 +++ t2,h1+++h2)
+        | I e1 a e2 =>
+          let '(e1 , t1, h1) := (rxcnf (negb polarity) e1) in
+          if polarity
+          then
+            if is_ff_no_deps_id e1 t1 h1
+            then (* e1 == cnf_ff and uses nothing *)
+              rxcnf polarity e2
+            else (* compute disjunction *)
+              let '(e2 , t2, h2) := (rxcnf polarity e2) in
+              let (f',t') := ror_cnf_opt e1 e2 in
+              (f', t1 +++ t2 +++ t',ocons a (h1+++h2)) (* record the hypothesis *)
+          else
+            let '(e2 , t2, h2) := (rxcnf polarity e2) in
+            (and_cnf_opt e1 e2, t1 +++ t2,h1+++h2)
+        end.
+      Proof.
+        destruct f ; reflexivity.
+      Qed.
 
       End CNFAnnot.
 
@@ -501,6 +576,17 @@ Section S.
         reflexivity.
       Qed.
 
+      Lemma ror_opt_cnf_cnf : forall f1 f2, fst (ror_cnf_opt f1 f2) = or_cnf_opt f1 f2.
+      Proof.
+        unfold ror_cnf_opt, or_cnf_opt.
+        intros.
+        destruct (is_cnf_tt f1).
+        - simpl ; auto.
+        - simpl. destruct (is_cnf_tt f2) ; simpl ; auto.
+          apply ror_cnf_cnf.
+      Qed.
+
+
       Lemma is_ff_no_deps_id_ff : forall T f d1 (d2 :list T),
           is_ff_no_deps_id f d1 d2 = true -> f = nil::nil.
       Proof.
@@ -517,6 +603,32 @@ Section S.
         congruence.
       Qed.
 
+      Lemma is_cnf_tt_inv : forall f1,
+          is_cnf_tt f1 = true -> f1 = cnf_tt.
+      Proof.
+        unfold cnf_tt.
+        destruct f1 ; simpl ; try congruence.
+      Qed.
+
+      Lemma is_cnf_ff_inv : forall f1,
+          is_cnf_ff f1 = true -> f1 = cnf_ff.
+      Proof.
+        unfold cnf_ff.
+        destruct f1 ; simpl ; try congruence.
+        destruct c ; simpl ; try congruence.
+        destruct f1 ; try congruence.
+        reflexivity.
+      Qed.
+
+      Lemma ratom_cnf : forall {AF : Type} f a,
+          fst (fst (ratom (AF:=AF) f a)) = f.
+      Proof.
+        unfold ratom.
+        intros.
+        destruct (is_cnf_ff f || is_cnf_tt f); auto.
+      Qed.
+
+
 
       Lemma rxcnf_xcnf : forall {TX AF:Type} (f:TFormula TX AF) b,
         fst (fst (rxcnf  b f)) = xcnf b f.
@@ -525,6 +637,7 @@ Section S.
         - destruct b; simpl ; auto.
         - destruct b; simpl ; auto.
         - destruct b ; simpl ; auto.
+        - intros. rewrite ratom_cnf. reflexivity.
         - intros.
           specialize (IHf1 b).
           specialize (IHf2 b).
@@ -532,8 +645,8 @@ Section S.
           destruct (rxcnf b f2).
           simpl in *. destruct p ; destruct p0; simpl in *.
           subst. destruct b ; auto.
-          rewrite <- ror_cnf_cnf.
-          destruct (ror_cnf (xcnf false f1) (xcnf false f2)).
+          rewrite <- ror_opt_cnf_cnf.
+          destruct (ror_cnf_opt (xcnf false f1) (xcnf false f2)).
           reflexivity.
         - intros.
           specialize (IHf1 b).
@@ -545,8 +658,8 @@ Section S.
           simpl in *.
           simpl in *. destruct p ; destruct p0; simpl in *.
           subst. destruct b ; auto.
-          rewrite <- ror_cnf_cnf.
-          destruct (ror_cnf (xcnf true f1) (xcnf true f2)).
+          rewrite <- ror_opt_cnf_cnf.
+          destruct (ror_cnf_opt (xcnf true f1) (xcnf true f2)).
           reflexivity.
         - intros.
           specialize (IHf1 (negb b)).
@@ -556,17 +669,20 @@ Section S.
           destruct (rxcnf (negb b) f1).
           destruct (rxcnf b f2).
           simpl in *.
-          simpl in *. destruct p ; destruct p0; simpl in *.
+          destruct p ; destruct p0; simpl in *.
           subst.
           destruct b;auto.
           generalize (is_ff_no_deps_id_ff (xcnf (negb true) f1) l1 l).
           destruct (is_ff_no_deps_id (xcnf (negb true) f1) l1 l).
           + intros.
             rewrite H by auto.
-            simpl. auto.
+            unfold or_cnf_opt.
+            simpl.
+            destruct (is_cnf_tt (xcnf true f2)) eqn:EQ;auto.
+            apply is_cnf_tt_inv in EQ; auto.
           +
-            rewrite <- ror_cnf_cnf.
-            destruct (ror_cnf (xcnf (negb true) f1) (xcnf true f2)).
+            rewrite <- ror_opt_cnf_cnf.
+            destruct (ror_cnf_opt (xcnf (negb true) f1) (xcnf true f2)).
             intros.
             reflexivity.
       Qed.
@@ -584,8 +700,9 @@ Section S.
 
 
 
-    Variable deduce_prop : forall env t t' u,
-        eval' env t -> eval' env t' -> deduce t t' = Some u -> eval' env u.
+    Variable deduce_prop : forall t t' u,
+        deduce t t' = Some u -> forall env,
+        eval' env t -> eval' env t' -> eval' env u.
 
 
 
@@ -597,13 +714,53 @@ Section S.
     Definition eval_cnf (env : Env) (f:cnf) := make_conj  (eval_clause  env) f.
 
 
-    Lemma eval_cnf_app : forall env x y, eval_cnf env (x+++y) -> eval_cnf env x /\ eval_cnf env y.
+    Lemma eval_cnf_app : forall env x y, eval_cnf env (x+++y) <-> eval_cnf env x /\ eval_cnf env y.
     Proof.
       unfold eval_cnf.
       intros.
-      rewrite make_conj_rapp in H.
-      rewrite make_conj_app in H ; auto.
+      rewrite make_conj_rapp.
+      rewrite make_conj_app ; auto.
+      tauto.
     Qed.
+
+
+    Lemma eval_cnf_ff : forall env, eval_cnf env cnf_ff <-> False.
+    Proof.
+      unfold cnf_ff, eval_cnf,eval_clause.
+      simpl. tauto.
+    Qed.
+
+    Lemma eval_cnf_tt : forall env, eval_cnf env cnf_tt <-> True.
+    Proof.
+      unfold cnf_tt, eval_cnf,eval_clause.
+      simpl. tauto.
+    Qed.
+
+
+    Lemma eval_cnf_and_opt : forall env x y, eval_cnf env (and_cnf_opt x y) <-> eval_cnf env (and_cnf x y).
+    Proof.
+      unfold and_cnf_opt.
+      intros.
+      destruct (is_cnf_ff x) eqn:F1.
+      { apply is_cnf_ff_inv in F1.
+        simpl. subst.
+        unfold and_cnf.
+        rewrite eval_cnf_app.
+        rewrite eval_cnf_ff.
+        tauto.
+      }
+      simpl.
+      destruct (is_cnf_ff y) eqn:F2.
+      { apply is_cnf_ff_inv in F2.
+        simpl. subst.
+        unfold and_cnf.
+        rewrite eval_cnf_app.
+        rewrite eval_cnf_ff.
+        tauto.
+      }
+      tauto.
+    Qed.
+
 
 
     Definition eval_opt_clause (env : Env) (cl: option clause) :=
@@ -613,57 +770,50 @@ Section S.
       end.
 
 
-  Lemma add_term_correct : forall env t cl , eval_opt_clause env (add_term t cl) -> eval_clause env (t::cl).
+  Lemma add_term_correct : forall env t cl , eval_opt_clause env (add_term t cl) <-> eval_clause env (t::cl).
   Proof.
     induction cl.
     - (* BC *)
     simpl.
-    case_eq (deduce (fst t) (fst t)) ; auto.
-    intros *.
-    case_eq (unsat t0) ; auto.
-    unfold eval_clause.
-    rewrite make_conj_cons.
-    intros. intro.
-    apply unsat_prop with (1:= H) (env := env).
-    apply deduce_prop with (3:= H0) ; tauto.
+    case_eq (deduce (fst t) (fst t)) ; try tauto.
+    intros.
+    generalize (@deduce_prop _ _ _ H env).
+    case_eq (unsat t0) ; try tauto.
+    { intros.
+      generalize (@unsat_prop _ H0 env).
+      unfold eval_clause.
+      rewrite make_conj_cons.
+      simpl; intros.
+      tauto.
+    }
     - (* IC *)
     simpl.
-    case_eq (deduce (fst t) (fst a)).
-    intro u.
-    case_eq (unsat u).
-    simpl. intros.
-    unfold eval_clause.
-    intro.
-    apply unsat_prop  with (1:= H) (env:= env).
-    repeat rewrite make_conj_cons in H2.
-    apply deduce_prop with (3:= H0); tauto.
-    intro.
-    case_eq (add_term t cl) ; intros.
-    simpl in H2.
-    rewrite H0 in IHcl.
-    simpl in IHcl.
-    unfold eval_clause in *.
+    case_eq (deduce (fst t) (fst a));
     intros.
-    repeat rewrite make_conj_cons in *.
-    tauto.
-    rewrite H0 in IHcl ; simpl in *.
-    unfold eval_clause in *.
-    intros.
-    repeat rewrite make_conj_cons in *.
-    tauto.
-    case_eq (add_term t cl) ; intros.
-    simpl in H1.
-    unfold eval_clause in *.
-    repeat rewrite make_conj_cons in *.
-    rewrite H in IHcl.
-    simpl in IHcl.
-    tauto.
-    simpl in *.
-    rewrite H in IHcl.
-    simpl in IHcl.
-    unfold eval_clause in *.
-    repeat rewrite make_conj_cons in *.
-    tauto.
+    generalize (@deduce_prop _ _ _ H env).
+    case_eq (unsat t0); intros.
+    {
+      generalize (@unsat_prop _ H0 env).
+      simpl.
+      unfold eval_clause.
+      repeat rewrite make_conj_cons.
+      tauto.
+    }
+    destruct (add_term t cl) ; simpl in * ; try tauto.
+    {
+      intros.
+      unfold eval_clause in *.
+      repeat rewrite make_conj_cons in *.
+      tauto.
+    }
+    {
+      unfold eval_clause in *.
+      repeat rewrite make_conj_cons in *.
+      tauto.
+    }
+    destruct (add_term t cl) ; simpl in *;
+      unfold eval_clause in * ;
+      repeat rewrite make_conj_cons in *; tauto.
   Qed.
 
 
@@ -676,41 +826,27 @@ Section S.
 
   Hint Resolve no_middle_eval_tt : tauto.
 
-  Lemma or_clause_correct : forall cl cl' env,  eval_opt_clause env (or_clause cl cl') -> eval_clause env cl \/ eval_clause env cl'.
+  Lemma or_clause_correct : forall cl cl' env,  eval_opt_clause env (or_clause cl cl') <-> eval_clause env cl \/ eval_clause env cl'.
   Proof.
     induction cl.
-    - simpl. tauto.
+    - simpl. unfold eval_clause at 2.  simpl. tauto.
     - intros *.
       simpl.
       assert (HH := add_term_correct env a cl').
-      case_eq (add_term a cl').
+      assert (eval_tt env a \/ ~ eval_tt env a) by (apply no_middle_eval').
+      destruct (add_term a cl'); simpl in *.
       +
-      intros.
-      apply IHcl in H0.
-      rewrite H in HH.
-      simpl in HH.
+      rewrite IHcl.
       unfold eval_clause in *.
-      destruct H0.
-      *
-      repeat rewrite make_conj_cons in *.
+      rewrite !make_conj_cons in *.
       tauto.
-      * apply HH in H0.
-        apply not_make_conj_cons in H0 ; auto with tauto.
+      + unfold eval_clause in *.
         repeat rewrite make_conj_cons in *.
         tauto.
-      +
-      intros.
-      rewrite H in HH.
-      simpl in HH.
-      unfold eval_clause in *.
-      assert (HH' := HH Coq.Init.Logic.I).
-      apply not_make_conj_cons in HH'; auto with tauto.
-      repeat rewrite make_conj_cons in *.
-      tauto.
   Qed.
 
 
-  Lemma or_clause_cnf_correct : forall env t f, eval_cnf env (or_clause_cnf t f) -> (eval_clause env t) \/ (eval_cnf env f).
+  Lemma or_clause_cnf_correct : forall env t f, eval_cnf env (or_clause_cnf t f) <-> (eval_clause env t) \/ (eval_cnf env f).
   Proof.
     unfold eval_cnf.
     unfold or_clause_cnf.
@@ -721,38 +857,53 @@ Section S.
                  | None => acc
                  end)).
     intro f.
-    assert (  make_conj (eval_clause env) (fold_left F f nil) -> (eval_clause env t \/ make_conj (eval_clause env) f) /\ make_conj (eval_clause env) nil).
+    assert (  make_conj (eval_clause env) (fold_left F f nil) <-> (eval_clause env t \/ make_conj (eval_clause env) f) /\ make_conj (eval_clause env) nil).
     {
       generalize (@nil clause) as acc.
       induction f.
       - simpl.
         intros ; tauto.
       - intros.
-        simpl in H.
-        apply IHf in H.
-        clear IHf.
-        destruct H.
+        simpl fold_left.
+        rewrite IHf.
         rewrite make_conj_cons.
         unfold F in *; clear F.
         generalize (or_clause_correct t a env).
         destruct (or_clause t a).
-        rewrite make_conj_cons in H0.
+        +
+        rewrite make_conj_cons.
         simpl. tauto.
-        simpl. tauto.
+        + simpl. tauto.
     }
     destruct t ; auto.
-    tauto.
+    - unfold eval_clause ; simpl. tauto.
+    - unfold xor_clause_cnf.
+      unfold F in H.
+      rewrite H.
+      unfold make_conj at 2. tauto.
   Qed.
 
 
-  Lemma eval_cnf_cons : forall env a f,  (~ make_conj  (eval_tt env) a) -> eval_cnf env f -> eval_cnf env (a::f).
+  Lemma eval_cnf_cons : forall env a f,  (~ make_conj  (eval_tt env) a  /\ eval_cnf env f) <-> eval_cnf env (a::f).
   Proof.
     intros.
     unfold eval_cnf in *.
     rewrite make_conj_cons ; eauto.
+    unfold eval_clause at 2.
+    tauto.
   Qed.
 
-  Lemma or_cnf_correct : forall env f f', eval_cnf env (or_cnf f f') -> (eval_cnf env  f) \/ (eval_cnf  env f').
+  Lemma eval_cnf_cons_iff : forall env a f,  ((~ make_conj  (eval_tt env) a) /\ eval_cnf env f) <-> eval_cnf env (a::f).
+  Proof.
+    intros.
+    unfold eval_cnf in *.
+    rewrite make_conj_cons ; eauto.
+    unfold eval_clause.
+    tauto.
+  Qed.
+
+
+  Lemma or_cnf_correct : forall env f f', eval_cnf env (or_cnf f f') <-> (eval_cnf env  f) \/ (eval_cnf  env f').
   Proof.
     induction f.
     unfold eval_cnf.
@@ -760,16 +911,40 @@ Section S.
     tauto.
     (**)
     intros.
-    simpl in H.
-    destruct (eval_cnf_app _ _ _ H).
-    clear H.
-    destruct (IHf _ H0).
-    destruct (or_clause_cnf_correct _ _ _ H1).
-    left.
-    apply eval_cnf_cons ; auto.
-    right ; auto.
-    right ; auto.
+    simpl.
+    rewrite eval_cnf_app.
+    rewrite <- eval_cnf_cons_iff.
+    rewrite IHf.
+    rewrite or_clause_cnf_correct.
+    unfold eval_clause.
+    tauto.
   Qed.
+
+  Lemma or_cnf_opt_correct : forall env f f', eval_cnf env (or_cnf_opt f f') <-> eval_cnf env (or_cnf f f').
+  Proof.
+    unfold or_cnf_opt.
+    intros.
+    destruct (is_cnf_tt f) eqn:TF.
+    { simpl.
+      apply is_cnf_tt_inv in TF.
+      subst.
+      rewrite or_cnf_correct.
+      rewrite eval_cnf_tt.
+      tauto.
+    }
+    destruct (is_cnf_tt f') eqn:TF'.
+    { simpl.
+      apply is_cnf_tt_inv in TF'.
+      subst.
+      rewrite or_cnf_correct.
+      rewrite eval_cnf_tt.
+      tauto.
+    }
+    { simpl. tauto. }
+  Qed.
+
+
+
 
   Variable normalise_correct : forall env t tg, eval_cnf  env (normalise t tg) -> eval env t.
 
@@ -778,16 +953,16 @@ Section S.
   Lemma xcnf_correct : forall (f : @GFormula Term Prop Annot unit)  pol env, eval_cnf env (xcnf pol f) -> eval_f (fun x => x) (eval env) (if pol then f else N f).
   Proof.
     induction f.
-    (* TT *)
+    - (* TT *)
     unfold eval_cnf.
     simpl.
     destruct pol ; simpl ; auto.
-    (* FF *)
+    - (* FF *)
     unfold eval_cnf.
     destruct pol; simpl ; auto.
     unfold eval_clause ; simpl.
     tauto.
-    (* P *)
+    - (* P *)
     simpl.
     destruct pol ; intros ;simpl.
     unfold eval_cnf in H.
@@ -799,7 +974,7 @@ Section S.
     unfold eval_cnf in H;simpl in H.
     unfold eval_clause in H ; simpl in H.
     tauto.
-    (* A *)
+    - (* A *)
     simpl.
     destruct pol ; simpl.
     intros.
@@ -807,49 +982,54 @@ Section S.
     (* A 2 *)
     intros.
     eapply  negate_correct ; eauto.
-    auto.
-    (* Cj *)
+    - (* Cj *)
     destruct pol ; simpl.
-    (* pol = true *)
+    + (* pol = true *)
     intros.
+    rewrite eval_cnf_and_opt in H.
     unfold and_cnf in H.
-    destruct (eval_cnf_app  _ _ _ H).
-    clear H.
+    rewrite eval_cnf_app  in H.
+    destruct H.
     split.
-    apply (IHf1 _ _ H0).
-    apply (IHf2 _ _ H1).
-    (* pol = false *)
+    apply (IHf1 _ _ H).
+    apply (IHf2 _ _ H0).
+    +  (* pol = false *)
     intros.
-    destruct (or_cnf_correct _ _ _ H).
-    generalize (IHf1 false  env H0).
+    rewrite or_cnf_opt_correct in H.
+    rewrite or_cnf_correct in H.
+    destruct H as [H | H].
+    generalize (IHf1 false  env H).
     simpl.
     tauto.
-    generalize (IHf2 false  env H0).
+    generalize (IHf2 false  env H).
     simpl.
     tauto.
-    (* D *)
+    - (* D *)
     simpl.
     destruct pol.
-    (* pol = true *)
+    + (* pol = true *)
     intros.
-    destruct (or_cnf_correct _ _ _ H).
-    generalize (IHf1 _  env H0).
+    rewrite or_cnf_opt_correct in H.
+    rewrite or_cnf_correct in H.
+    destruct H as [H | H].
+    generalize (IHf1 _  env H).
     simpl.
     tauto.
-    generalize (IHf2 _  env H0).
+    generalize (IHf2 _  env H).
     simpl.
     tauto.
-    (* pol = true *)
+    + (* pol = true *)
+    intros.
+    rewrite eval_cnf_and_opt in H.
     unfold and_cnf.
-    intros.
-    destruct (eval_cnf_app  _ _ _ H).
-    clear H.
+    rewrite eval_cnf_app in H.
+    destruct H as [H0 H1].
     simpl.
     generalize (IHf1 _ _ H0).
     generalize (IHf2 _ _ H1).
     simpl.
     tauto.
-    (**)
+    - (**)
     simpl.
     destruct pol ; simpl.
     intros.
@@ -857,25 +1037,29 @@ Section S.
     intros.
     generalize (IHf _ _ H).
     tauto.
-    (* I *)
+    - (* I *)
     simpl; intros.
     destruct pol.
-    simpl.
+    + simpl.
     intro.
-    destruct (or_cnf_correct _ _ _ H).
-    generalize (IHf1 _ _ H1).
+    rewrite or_cnf_opt_correct in H.
+    rewrite or_cnf_correct in H.
+    destruct H as [H | H].
+    generalize (IHf1 _ _ H).
     simpl in *.
     tauto.
-    generalize (IHf2 _ _ H1).
+    generalize (IHf2 _ _ H).
     auto.
-    (* pol = false *)
-    unfold and_cnf in H.
-    simpl in H.
-    destruct (eval_cnf_app _ _ _ H).
-    generalize (IHf1 _ _ H0).
-    generalize (IHf2 _ _ H1).
-    simpl.
-    tauto.
+    + (* pol = false *)
+      rewrite eval_cnf_and_opt in H.
+      unfold and_cnf in H.
+      simpl in H.
+      rewrite eval_cnf_app in H.
+      destruct H as [H0 H1].
+      generalize (IHf1 _ _ H0).
+      generalize (IHf2 _ _ H1).
+      simpl.
+      tauto.
   Qed.
 
 
